To prove $p \not\equiv q$, use counterexample
To prove $p \equiv q$, use truth table if not exactly logically equivalent

## Definition

| Term | Definition |
| --- | --- |
| Negation | If p is a statement variable, the negation of p is "not p" or "it is not the case that p" and is denoted $\sim p$. |
| Conjunction | "p and q", denoted $p \land q$ |
| Disjunction | "p or q", denoted $p \lor q$ |
| Logical Equivalence | Two statement forms are called logically equivalent if, and only if, they have identical truth values for each possible substitution of statements for their statement variables. The logical equivalence of statement forms P and Q is denoted by $P \equiv Q$ |
| Tautology | Statement form that is always true |
| Contradiction | Always false regardless of truth values |

## Logical Equivalences

Given statement variables p, q, r and a tautology "true", and a contradiction "false".

| Law                     | Equivalent Expression                            | Alternate Equivalence                |
|-------------------------|---------------------------------------|--------------------------------------|
| Commutative laws        | $p \land q \equiv q \land p$           | $p \lor q \equiv q \lor p$           |
| Associative laws        | $(p \lor q) \lor r \equiv p \lor (q \lor r)$                   | $(p \land q) \land r \equiv p \land (q \land r)$ |
| Distributive laws       | $p \land (q \lor r) \equiv (p \land q) \lor (p \land r)$ | $p \lor (q \land r) \equiv (p \lor q) \land (p \lor r)$ |
| Identity laws           | $p \land \text{true} \equiv p$         | $p \lor \text{false} \equiv p$       |
| Negation laws           | $p \lor \sim p \equiv \text{true}$    | $p \land \sim p \equiv \text{false}$ |
| Double negative law     | $\sim (\sim p) \equiv p$              |                                      |
| Idempotent laws         | $p \land p \equiv p$                  | $p \lor p \equiv p$                  |
| Universal bound laws    | $p \lor \text{true} \equiv \text{true}$ | $p \land \text{false} \equiv \text{false}$ |
| De Morganâ€™s laws        | $\sim (p \land q) \equiv \sim p \lor \sim q$ | $\sim (p \lor q) \equiv \sim p \land \sim q$ |
| Absorption laws         | $p \lor (p \land q) \equiv p$         | $p \land (p \lor q) \equiv p$       |
| Negation of true and false | $\sim \text{true} \equiv \text{false}$ | $\sim \text{false} \equiv \text{true}$ |


## Conditionals

|Term|Definition|
|---|---|
| Conditional | If p then q, or p implies q. Denoted by $p \rightarrow q$. p is the hypothesis and q the conclusion |
| Contrapositive | The contrapositive of a conditional statement $p \rightarrow q$ is $\sim q \rightarrow \sim p$ |
| Converse | The converse of $p \rightarrow q$ is $q \rightarrow p$ |
| Inverse | The inverse of $p \rightarrow q$ is $\sim p \rightarrow \sim q$ |
| Only if | "p only if q" means "if not q then not p" ($\sim q \rightarrow \sim p$). Alternate: "if p then q", $p \rightarrow q$ |
| Biconditional | "p if, and only if (iff), q", denoted by $p \iff q$. True if both p and q have the same values and is false if p and q have opposite truth values |
| Sufficient Condition | r is a sufficient condition for s: "if r then s" or $r \rightarrow s$ |
| Necessary Condition | r is a necessary condition for s: "if not r then not s" or "if s then r" or $s \rightarrow r$


### Rules
| Law | Equivalent Expression |
| --- | --- |
| Implication Law | $p \rightarrow q \equiv \sim p \lor q$ |
| Conditional = Contrapositive | $p \rightarrow q \equiv \sim q \rightarrow \sim p$ |
| Converse = Inverse | $q \rightarrow p \equiv \sim p \rightarrow \sim q$ |
| Transitive Rule of Inference | $((p \rightarrow q) \land (q \rightarrow r)) \implies (p \rightarrow r)$ |

HOWEVER, $p \rightarrow q \not\equiv q \rightarrow p$


## Truth Table of Conditional

Using $p \implies q$

| p | q | $p \implies q$ |
|:---:|:---:|:---:|
| T | T | T |
| T | F | F |
| F | T | T |
| F | F | T |

