## Definitions
- $n$ is odd $\iff$ $n=2k$
- $n$ is even $\iff$ $n=2k+1$
- Prime
	- More than 1 and either r or s is n where n=rs
	- $(n > 1) \land \forall r,s \in \mathbb{Z}^+, (n=rs \implies (r=1\land s= n)\lor(r = n\land s = 1))$
- Composite
	- $\exists r,s \in \mathbb{Z}^+ (n=rs\land (1<r<n) \land (1<s<n))$

## Proofs

### Direct Proofs
Example: Prove that the product of 2 consecutive odd numbers is always odd
```
1. Let a and b be the two consecutive odd numbers.
   1.1 Without loss of generality, assume that a < b, hence b = a + 2.
   1.2 Now, a = 2k + 1 for some integer k (by definition of odd numbers).
   1.3 Similarly, b = a + 2 = 2k + 3.
   1.4 Therefore, ab = (2k + 1)(2k + 3) = 4k^2 + 2k + 6k + 3 = 4k^2 + 8k + 3 = 2(2k^2 + 4k) + 1 + 1 (by basic algebra).
   1.5 Let m = 2k, then ab = 2m + 1 which is an integer (by closure of integers under multiplication and addition).
   1.6 Then ab = 2m + 1, which is odd (by definition of odd numbers).
2. Therefore, the product of two consecutive odd numbers is always odd.
```

#### Proof by Construction
- Form of direct proof
- "Plug in a number and prove"

Prove that there exists $x \in \mathbb{Z}\ s.t.\ x > 2\ and\ x^2 -5x + 6 > 0$
```
1. Let x = 17
2. Note that 17 is an integer and 17 > 2
3. x^2 -5x + 6 = 210 > 0
```
#### Proof by Exhaustion
- "Plug all possible numbers"
- E.g. Prove that 6a is not divisible by 5 for an integer a between 1 and 4 inclusive --> Test a=1 to a=4

#### Proof by Deduction
- Used for infinite cases

**E.g. Prove that the difference of two consecutive squares is always odd**
> 1. Let the numbers be n and n + 1
		1.1 $(n+1)^2 - n^2 = 2n + 1$ (by basic algebra)
		1.2 $2n + 1$ is odd (by definition of odd numbers)
    2. Therefore the difference between 2 consecutive squares is odd

#### Proof by Contradiction
- To prove statement S, assume ~S (not S) is true
- Use facts and theorems to arrive at logical contradiction
- Since every step is logical, problem lies in assumption that ~S is true
- Conclude ~S is false $\implies$ S is true

**E.g. Prove that $\sqrt{2}$ is rational**
> 1. Suppose not, that is, $2$ is rational. 
> 	1.1 Then $\exists\ a,\ b \in \mathbb{Z}$, $b \neq 0$ s.t. $2 = \frac{a}{b}$ (by definition of rational numbers) 
> 	1.2 Convert $\frac{a}{b}$ to its lowest term $\frac{m}{n}$. 
> 	1.3 $m^2 = 2n^2$ (by basic algebra) 
> 	1.4 Hence $m^2$ is even (by definition of even number, as $n^2$ is an integer by closure) 
> 	1.5 Hence $m$ is even (by Proposition 4.6.4) 
> 	1.6 Let $m = 2k$; substituting into 1.3: $4k^2 = 2n^2$, or $n^2 = 2k^2$ 
> 	1.7 Hence $n^2$ is even (by definition of even number) 
> 	1.8 Hence $n$ is even (by Proposition 4.6.4) 
> 	1.9 So both $m$ and $n$ are even, but this contradicts that $\frac{m}{n}$ is in its lowest term. 
>  2. Therefore, the assumption that $2$ is rational is false. 
>  3. Hence $2$ is irrational.

#### Proof by Cases

**Example: Prove that there are irrational numbers p and q where $p^q$ is rational**
> 1. From previous theorem, $\sqrt{2}$ is irrational
> 2.  Consider $\sqrt{2}^\sqrt{2}$. This can be rational or irrational
> 3. Case 1: $\sqrt{2}^\sqrt{2}$ is rational
> 	3.1. Let $p = q = \sqrt{2}$, and we are done
> 4. Case 2: $\sqrt{2}^\sqrt{2}$ is irrational
> 	4.1. Let $p = \sqrt{2}^\sqrt{2}$ and $q = \sqrt{2}$
> 	4.2 Now $p$ is irrational (by assumption) and so is $q$ (by previous theorem)
> 	4.3 Consider $p^q = (\sqrt{2}^\sqrt{2})^\sqrt{2} = \sqrt{2}^{(\sqrt{2}\sqrt{2})} = \sqrt{2}^2 = 2$ (By algebra)
> 	4.4 2 is rational
> 5. IN either case we have found the required $p$ and $q$

#### Universal & Existential Statements
- To prove existential, prove by example
- Or disprove universal by counterexample

### Indirect Proofs
#### Proof by Contradiction
- Suppose statement S is false: Negation of S is true
- Show it leads to logical contradiction
- Conclude S is true

#### Proof by Contraposition
- For $p \implies q$, prove $\sim q \implies \sim p$